rocq/theories/TypeSystem/EnvRuntimeBaseSafety.v
@@ -16736,6 +16736,8 @@ Definition callee_body_root_shadow_captured_call_generic_direct_narrow_store_saf
     Datatypes.length type_args = fn_type_params fcallee /\
     check_struct_bounds (global_env_with_local_bounds env (fn_bounds fdef))
       (fn_bounds fcallee) type_args = None /\
+    preservation_ready_expr
+      (subst_type_params_expr type_args (fn_body fcallee)) /\
     callee_body_root_shadow_store_safe_narrow_summary_instantiated_fuel
       env 10000 fcallee type_args /\
     NoDup (ctx_names (params_ctx (fn_params fdef))) /\
@@ -16876,7 +16878,7 @@ Proof.
   destruct Hsummary as
     (fname & type_args & args & raw_body & synthetic_body & fcallee &
       T_body & Gamma_out & R_body & roots_body & Hbody & Htarget &
-      Hsynthetic & Hsafe & Hin & Hname & Harity & Hbounds &
+      Hsynthetic & Hsafe & Hin & Hname & Harity & Hbounds & Hcallee_ready &
       Hcallee_summary & Hnodup & Htyped & Hcompat & Hexcl_roots & Hexcl_env).
   eapply CBRSSNI_GenericDirect with
     (raw_body := raw_body) (synthetic_body := synthetic_body)
@@ -16966,7 +16968,7 @@ Proof.
     eqn:Hbody_env; try discriminate.
   repeat rewrite andb_true_iff in Hgeneric.
   destruct Hgeneric as
-    [[[[[[Hcallee_expr Hcallee_compat] Hcallee_roots]
+    [[[[[[[Hcallee_ready Hcallee_expr] Hcallee_compat] Hcallee_roots]
          Hcallee_env_excl] Hcompat] Hroots] Henv].
   apply lookup_fn_b_sound in Hlookup_b.
   destruct Hlookup_b as [Hin_callee Hname_callee].
@@ -16992,6 +16994,8 @@ Proof.
   split; [exact Hname_callee |].
   split; [exact Htype_params |].
   split; [exact Hbounds |].
+  split.
+  { apply preservation_ready_expr_b_sound. exact Hcallee_ready. }
   split; [exact Hcallee_summary |].
   split.
   { change (NoDup
